theories/interpreter_func.v
@@ -80,11 +80,11 @@ Definition depth := nat.
 
 Definition fuel := nat.
 
-Definition config_tuple := ((host_state * store_record * list value * list administrative_instruction)%type).
+Definition config_tuple := ((host_state * store_record * frame * list administrative_instruction)%type).
 
-Definition config_one_tuple_without_e := (host_state * store_record * list value * list value)%type.
+Definition config_one_tuple_without_e := (host_state * store_record * frame * list value)%type.
 
-Definition res_tuple := (host_state * store_record * list value * res_step)%type.
+Definition res_tuple := (host_state * store_record * frame * res_step)%type.
 (*
 Fixpoint split_vals (es : list basic_instruction) : ((list value) * (list basic_instruction))%type :=
   match es with
@@ -151,320 +151,320 @@ Proof.
   - move=> >. by apply: ReflectF.
 Qed.*)
 
-Fixpoint run_step_with_fuel (fuel : fuel) (d : depth) (i : instance) (cfg : config_tuple) : res_tuple :=
-  let: (hs, s, vs, es) := cfg in
+Fixpoint run_step_with_fuel (fuel : fuel) (d : depth) (cfg : config_tuple) : res_tuple :=
+  let: (hs, s, f, es) := cfg in
   match fuel with
-  | 0 => (hs, s, vs, RS_crash C_exhaustion)
+  | 0 => (hs, s, f, RS_crash C_exhaustion)
   | fuel.+1 =>
     let: (ves, es') := split_vals_e es in (** Framing out constants. **)
     match es' with
-    | [::] => (hs, s, vs, crash_error)
+    | [::] => (hs, s, f, crash_error)
     | e :: es'' =>
       if e_is_trap e
       then
         if (es'' != [::]) || (ves != [::])
-        then (hs, s, vs, RS_normal [::Trap])
-        else (hs, s, vs, crash_error)
+        then (hs, s, f, RS_normal [::Trap])
+        else (hs, s, f, crash_error)
       else
-        let: (hs', s', vs', r) := run_one_step fuel d i (hs, s, vs, (rev ves)) e in
+        let: (hs', s', f', r) := run_one_step fuel d (hs, s, f, (rev ves)) e in
         if r is RS_normal res
-        then (hs', s', vs', RS_normal (res ++ es''))
-        else (hs', s', vs', r)
+        then (hs', s', f', RS_normal (res ++ es''))
+        else (hs', s', f', r)
     end
   end
-
-with run_one_step (fuel : fuel) (d : depth) (i : instance) (cfg : config_one_tuple_without_e) (e : administrative_instruction) : res_tuple :=
-  let: (hs, s, vs, ves) := cfg in
+    
+with run_one_step (fuel : fuel) (d : depth) (cfg : config_one_tuple_without_e) (e : administrative_instruction) : res_tuple :=
+  let: (hs, s, f, ves) := cfg in
   match fuel with
-  | 0 => (hs, s, vs, RS_crash C_exhaustion)
+  | 0 => (hs, s, f, RS_crash C_exhaustion)
   | fuel.+1 =>
     match e with
     (* unop *)
     | Basic (Unop t op) =>
       if ves is v :: ves' then
-        (hs, s, vs, RS_normal (vs_to_es (app_unop op v :: ves')))
-      else (hs, s, vs, crash_error)
+        (hs, s, f, RS_normal (vs_to_es (app_unop op v :: ves')))
+      else (hs, s, f, crash_error)
     (* binop *)
     | Basic (Binop t op) =>
       if ves is v2 :: v1 :: ves' then
         expect (app_binop op v1 v2)
-               (fun v => (hs, s, vs, RS_normal (vs_to_es (v :: ves'))))
-               (hs, s, vs, RS_normal ((vs_to_es ves') ++ [::Trap]))
-      else (hs, s, vs, crash_error)
+               (fun v => (hs, s, f, RS_normal (vs_to_es (v :: ves'))))
+               (hs, s, f, RS_normal ((vs_to_es ves') ++ [::Trap]))
+      else (hs, s, f, crash_error)
     (* testops *)
     | Basic (Testop T_i32 testop) =>
       if ves is (ConstInt32 c) :: ves' then
-        (hs, s, vs, RS_normal (vs_to_es ((ConstInt32 (wasm_bool (@app_testop_i i32t testop c))) :: ves')))
-      else (hs, s, vs, crash_error)
+        (hs, s, f, RS_normal (vs_to_es ((ConstInt32 (wasm_bool (@app_testop_i i32t testop c))) :: ves')))
+      else (hs, s, f, crash_error)
     | Basic (Testop T_i64 testop) =>
       if ves is (ConstInt64 c) :: ves' then
-        (hs, s, vs, RS_normal (vs_to_es ((ConstInt32 (wasm_bool (@app_testop_i i64t testop c))) :: ves')))
-      else (hs, s, vs, crash_error)
-    | Basic (Testop _ _) => (hs, s, vs, crash_error)
+        (hs, s, f, RS_normal (vs_to_es ((ConstInt32 (wasm_bool (@app_testop_i i64t testop c))) :: ves')))
+      else (hs, s, f, crash_error)
+    | Basic (Testop _ _) => (hs, s, f, crash_error)
     (* relops *)
     | Basic (Relop t op) =>
       if ves is v2 :: v1 :: ves' then
-        (hs, s, vs, RS_normal (vs_to_es (ConstInt32 (wasm_bool (app_relop op v1 v2)) :: ves')))
-      else (hs, s, vs, crash_error)
+        (hs, s, f, RS_normal (vs_to_es (ConstInt32 (wasm_bool (app_relop op v1 v2)) :: ves')))
+      else (hs, s, f, crash_error)
     (* convert & reinterpret *)
     | Basic (Cvtop t2 Convert t1 sx) =>
       if ves is v :: ves' then
         if types_agree t1 v
         then
           expect (cvt t2 sx v) (fun v' =>
-               (hs, s, vs, RS_normal (vs_to_es (v' :: ves'))))
-            (hs, s, vs, RS_normal ((vs_to_es ves') ++ [::Trap]))
-        else (hs, s, vs, crash_error)
-      else (hs, s, vs, crash_error)
+               (hs, s, f, RS_normal (vs_to_es (v' :: ves'))))
+            (hs, s, f, RS_normal ((vs_to_es ves') ++ [::Trap]))
+        else (hs, s, f, crash_error)
+      else (hs, s, f, crash_error)
     | Basic (Cvtop t2 Reinterpret t1 sx) =>
       if ves is v :: ves' then
         if types_agree t1 v && (sx == None)
-        then (hs, s, vs, RS_normal (vs_to_es (wasm_deserialise (bits v) t2 :: ves')))
-        else (hs, s, vs, crash_error)
-      else (hs, s, vs, crash_error)
+        then (hs, s, f, RS_normal (vs_to_es (wasm_deserialise (bits v) t2 :: ves')))
+        else (hs, s, f, crash_error)
+      else (hs, s, f, crash_error)
     (**)
-    | Basic Unreachable => (hs, s, vs, RS_normal ((vs_to_es ves) ++ [::Trap]))
-    | Basic Nop => (hs, s, vs, RS_normal (vs_to_es ves))
+    | Basic Unreachable => (hs, s, f, RS_normal ((vs_to_es ves) ++ [::Trap]))
+    | Basic Nop => (hs, s, f, RS_normal (vs_to_es ves))
     | Basic Drop =>
       if ves is v :: ves' then
-        (hs, s, vs, RS_normal (vs_to_es ves'))
-      else (hs, s, vs, crash_error)
+        (hs, s, f, RS_normal (vs_to_es ves'))
+      else (hs, s, f, crash_error)
     | Basic Select =>
       if ves is (ConstInt32 c) :: v2 :: v1 :: ves' then
         if c == Wasm_int.int_zero i32m
-        then (hs, s, vs, RS_normal (vs_to_es (v2 :: ves')))
-        else (hs, s, vs, RS_normal (vs_to_es (v1 :: ves')))
-      else (hs, s, vs, crash_error)
+        then (hs, s, f, RS_normal (vs_to_es (v2 :: ves')))
+        else (hs, s, f, RS_normal (vs_to_es (v1 :: ves')))
+      else (hs, s, f, crash_error)
     | Basic (Block (Tf t1s t2s) es) =>
       if length ves >= length t1s
       then
         let: (ves', ves'')  := split_n ves (length t1s) in
-        (hs, s, vs, RS_normal (vs_to_es ves''
+        (hs, s, f, RS_normal (vs_to_es ves''
                 ++ [::Label (length t2s) [::] (vs_to_es ves' ++ to_e_list es)]))
-      else (hs, s, vs, crash_error)
+      else (hs, s, f, crash_error)
     | Basic (Loop (Tf t1s t2s) es) =>
       if length ves >= length t1s
       then
         let: (ves', ves'') := split_n ves (length t1s) in
-        (hs, s, vs, RS_normal (vs_to_es ves''
+        (hs, s, f, RS_normal (vs_to_es ves''
                 ++ [::Label (length t1s) [::Basic (Loop (Tf t1s t2s) es)]
                         (vs_to_es ves' ++ to_e_list es)]))
-      else (hs, s, vs, crash_error)
+      else (hs, s, f, crash_error)
     | Basic (If tf es1 es2) =>
       if ves is ConstInt32 c :: ves' then
         if c == Wasm_int.int_zero i32m
-        then (hs, s, vs, RS_normal (vs_to_es ves' ++ [::Basic (Block tf es2)]))
-        else (hs, s, vs, RS_normal (vs_to_es ves' ++ [::Basic (Block tf es1)]))
-      else (hs, s, vs, crash_error)
-    | Basic (Br j) => (hs, s, vs, RS_break j ves)
+        then (hs, s, f, RS_normal (vs_to_es ves' ++ [::Basic (Block tf es2)]))
+        else (hs, s, f, RS_normal (vs_to_es ves' ++ [::Basic (Block tf es1)]))
+      else (hs, s, f, crash_error)
+    | Basic (Br j) => (hs, s, f, RS_break j ves)
     | Basic (Br_if j) =>
       if ves is ConstInt32 c :: ves' then
         if c == Wasm_int.int_zero i32m
-        then (hs, s, vs, RS_normal (vs_to_es ves'))
-        else (hs, s, vs, RS_normal (vs_to_es ves' ++ [::Basic (Br j)]))
-      else (hs, s, vs, crash_error)
+        then (hs, s, f, RS_normal (vs_to_es ves'))
+        else (hs, s, f, RS_normal (vs_to_es ves' ++ [::Basic (Br j)]))
+      else (hs, s, f, crash_error)
     | Basic (Br_table js j) =>
       if ves is ConstInt32 c :: ves' then
         let: k := Wasm_int.nat_of_uint i32m c in
         if k < length js
         then
           expect (List.nth_error js k) (fun js_at_k =>
-              (hs, s, vs, RS_normal (vs_to_es ves' ++ [::Basic (Br js_at_k)])))
-            (hs, s, vs, crash_error)
-        else (hs, s, vs, RS_normal (vs_to_es ves' ++ [::Basic (Br j)]))
-      else (hs, s, vs, crash_error)
+              (hs, s, f, RS_normal (vs_to_es ves' ++ [::Basic (Br js_at_k)])))
+            (hs, s, f, crash_error)
+        else (hs, s, f, RS_normal (vs_to_es ves' ++ [::Basic (Br j)]))
+      else (hs, s, f, crash_error)
     | Basic (Call j) =>
-      if sfunc s i j is Some sfunc_i_j then
-        (hs, s, vs, RS_normal (vs_to_es ves ++ [::Invoke sfunc_i_j]))
-      else (hs, s, vs, crash_error)
+      if sfunc s f.(f_inst) j is Some sfunc_i_j then
+        (hs, s, f, RS_normal (vs_to_es ves ++ [::Invoke sfunc_i_j]))
+      else (hs, s, f, crash_error)
     | Basic (Call_indirect j) =>
       if ves is ConstInt32 c :: ves' then
-        match stab s i (Wasm_int.nat_of_uint i32m c) with
+        match stab s f.(f_inst) (Wasm_int.nat_of_uint i32m c) with
         | Some cl =>
-          if stypes s i j == Some (cl_type cl)
-          then (hs, s, vs, RS_normal (vs_to_es ves' ++ [::Invoke cl]))
-          else (hs, s, vs, RS_normal (vs_to_es ves' ++ [::Trap]))
-        | None => (hs, s, vs, RS_normal (vs_to_es ves' ++ [::Trap]))
+          if stypes s f.(f_inst) j == Some (cl_type cl)
+          then (hs, s, f, RS_normal (vs_to_es ves' ++ [::Invoke cl]))
+          else (hs, s, f, RS_normal (vs_to_es ves' ++ [::Trap]))
+        | None => (hs, s, f, RS_normal (vs_to_es ves' ++ [::Trap]))
         end
-      else (hs, s, vs, crash_error)
-    | Basic Return => (hs, s, vs, RS_return ves)
+      else (hs, s, f, crash_error)
+    | Basic Return => (hs, s, f, RS_return ves)
     | Basic (Get_local j) =>
-      if j < length vs
+      if j < length f.(f_locs)
       then
-        expect (List.nth_error vs j) (fun vs_at_j =>
-            (hs, s, vs, RS_normal (vs_to_es (vs_at_j :: ves))))
-          (hs, s, vs, crash_error)
-      else (hs, s, vs, crash_error)
+        expect (List.nth_error f.(f_locs) j) (fun vs_at_j =>
+            (hs, s, f, RS_normal (vs_to_es (vs_at_j :: ves))))
+          (hs, s, f, crash_error)
+      else (hs, s, f, crash_error)
     | Basic (Set_local j) =>
       if ves is v :: ves' then
-        if j < length vs
-        then (hs, s, update_list_at vs j v, RS_normal (vs_to_es ves'))
-        else (hs, s, vs, crash_error)
-      else (hs, s, vs, crash_error)
+        if j < length f.(f_locs)
+        then (hs, s, Build_frame (update_list_at f.(f_locs) j v) f.(f_inst), RS_normal (vs_to_es ves'))
+        else (hs, s, f, crash_error)
+      else (hs, s, f, crash_error)
     | Basic (Tee_local j) =>
       if ves is v :: ves' then
-        (hs, s, vs, RS_normal (vs_to_es (v :: ves) ++ [::Basic (Set_local j)]))
-      else (hs, s, vs, crash_error)
+        (hs, s, f, RS_normal (vs_to_es (v :: ves) ++ [::Basic (Set_local j)]))
+      else (hs, s, f, crash_error)
     | Basic (Get_global j) =>
-      if sglob_val s i j is Some xx
-      then (hs, s, vs, RS_normal (vs_to_es (xx :: ves)))
-      else (hs, s, vs, crash_error)
+      if sglob_val s f.(f_inst) j is Some xx
+      then (hs, s, f, RS_normal (vs_to_es (xx :: ves)))
+      else (hs, s, f, crash_error)
     | Basic (Set_global j) =>
       if ves is v :: ves' then
-        if supdate_glob s i j v is Some xx
-        then (hs, xx, vs, RS_normal (vs_to_es ves'))
-        else (hs, s, vs, crash_error)
-      else (hs, s, vs, crash_error)
+        if supdate_glob s f.(f_inst) j v is Some xx
+        then (hs, xx, f, RS_normal (vs_to_es ves'))
+        else (hs, s, f, crash_error)
+      else (hs, s, f, crash_error)
     | Basic (Load t None a off) =>
       if ves is ConstInt32 k :: ves' then
         expect
-          (smem_ind s i)
+          (smem_ind s f.(f_inst))
           (fun j =>
              if List.nth_error s.(s_mems) j is Some mem_s_j then
                expect
                  (load (mem_s_j) (Wasm_int.N_of_uint i32m k) off (t_length t))
-                 (fun bs => (hs, s, vs, RS_normal (vs_to_es (wasm_deserialise bs t :: ves'))))
-                 (hs, s, vs, RS_normal (vs_to_es ves' ++ [::Trap]))
-             else (hs, s, vs, crash_error))
-          (hs, s, vs, crash_error)
-      else (hs, s, vs, crash_error)
+                 (fun bs => (hs, s, f, RS_normal (vs_to_es (wasm_deserialise bs t :: ves'))))
+                 (hs, s, f, RS_normal (vs_to_es ves' ++ [::Trap]))
+             else (hs, s, f, crash_error))
+          (hs, s, f, crash_error)
+      else (hs, s, f, crash_error)
     | Basic (Load t (Some (tp, sx)) a off) =>
       if ves is ConstInt32 k :: ves' then
         expect
-          (smem_ind s i)
+          (smem_ind s f.(f_inst))
           (fun j =>
              if List.nth_error s.(s_mems) j is Some mem_s_j then
                expect
                  (load_packed sx (mem_s_j) (Wasm_int.N_of_uint i32m k) off (tp_length tp) (t_length t))
-                 (fun bs => (hs, s, vs, RS_normal (vs_to_es (wasm_deserialise bs t :: ves'))))
-                 (hs, s, vs, RS_normal (vs_to_es ves' ++ [::Trap]))
-             else (hs, s, vs, crash_error))
-          (hs, s, vs, crash_error)
-      else (hs, s, vs, crash_error)
+                 (fun bs => (hs, s, f, RS_normal (vs_to_es (wasm_deserialise bs t :: ves'))))
+                 (hs, s, f, RS_normal (vs_to_es ves' ++ [::Trap]))
+             else (hs, s, f, crash_error))
+          (hs, s, f, crash_error)
+      else (hs, s, f, crash_error)
     | Basic (Store t None a off) =>
       if ves is v :: ConstInt32 k :: ves' then
         if types_agree t v
         then
           expect
-            (smem_ind s i)
+            (smem_ind s f.(f_inst))
             (fun j =>
                if List.nth_error s.(s_mems) j is Some mem_s_j then
                  expect
                    (store mem_s_j (Wasm_int.N_of_uint i32m k) off (bits v) (t_length t))
                    (fun mem' =>
-                      (hs, upd_s_mem s (update_list_at s.(s_mems) j mem'), vs, RS_normal (vs_to_es ves')))
-                   (hs, s, vs, RS_normal (vs_to_es ves' ++ [::Trap]))
-               else (hs, s, vs, crash_error))
-            (hs, s, vs, crash_error)
-        else (hs, s, vs, crash_error)
-      else (hs, s, vs, crash_error)
+                      (hs, upd_s_mem s (update_list_at s.(s_mems) j mem'), f, RS_normal (vs_to_es ves')))
+                   (hs, s, f, RS_normal (vs_to_es ves' ++ [::Trap]))
+               else (hs, s, f, crash_error))
+            (hs, s, f, crash_error)
+        else (hs, s, f, crash_error)
+      else (hs, s, f, crash_error)
     | Basic (Store t (Some tp) a off) =>
       if ves is v :: ConstInt32 k :: ves' then
         if types_agree t v
         then
           expect
-            (smem_ind s i)
+            (smem_ind s f.(f_inst))
             (fun j =>
                if List.nth_error s.(s_mems) j is Some mem_s_j then
                  expect
                    (store_packed mem_s_j (Wasm_int.N_of_uint i32m k) off (bits v) (tp_length tp))
                    (fun mem' =>
-                      (hs, upd_s_mem s (update_list_at s.(s_mems) j mem'), vs, RS_normal (vs_to_es ves')))
-                   (hs, s, vs, RS_normal (vs_to_es ves' ++ [::Trap]))
-               else (hs, s, vs, crash_error))
-            (hs, s, vs, crash_error)
-        else (hs, s, vs, crash_error)
-      else (hs, s, vs, crash_error)
+                      (hs, upd_s_mem s (update_list_at s.(s_mems) j mem'), f, RS_normal (vs_to_es ves')))
+                   (hs, s, f, RS_normal (vs_to_es ves' ++ [::Trap]))
+               else (hs, s, f, crash_error))
+            (hs, s, f, crash_error)
+        else (hs, s, f, crash_error)
+      else (hs, s, f, crash_error)
     | Basic Current_memory =>
       expect
-        (smem_ind s i)
+        (smem_ind s f.(f_inst))
         (fun j =>
            if List.nth_error s.(s_mems) j is Some s_mem_s_j then
-             (hs, s, vs, RS_normal (vs_to_es (ConstInt32 (Wasm_int.int_of_Z i32m (Z.of_nat (mem_size s_mem_s_j))) :: ves)))
-           else (hs, s, vs, crash_error))
-        (hs, s, vs, crash_error)
+             (hs, s, f, RS_normal (vs_to_es (ConstInt32 (Wasm_int.int_of_Z i32m (Z.of_nat (mem_size s_mem_s_j))) :: ves)))
+           else (hs, s, f, crash_error))
+        (hs, s, f, crash_error)
     | Basic Grow_memory =>
       if ves is ConstInt32 c :: ves' then
         expect
-          (smem_ind s i)
+          (smem_ind s f.(f_inst))
           (fun j =>
             if List.nth_error s.(s_mems) j is Some s_mem_s_j then
               let: l := mem_size s_mem_s_j in
               let: mem' := mem_grow s_mem_s_j (Wasm_int.N_of_uint i32m c) in
               if mem' is Some mem'' then
-                (hs, upd_s_mem s (update_list_at s.(s_mems) j mem''), vs,
+                (hs, upd_s_mem s (update_list_at s.(s_mems) j mem''), f,
                  RS_normal (vs_to_es (ConstInt32 (Wasm_int.int_of_Z i32m (Z.of_nat l)) :: ves')))
-              else (hs, s, vs, crash_error)
-            else (hs, s, vs, crash_error))
-          (hs, s, vs, crash_error)
-      else (hs, s, vs, crash_error)
-    | Basic (EConst _) => (hs, s, vs, crash_error)
+              else (hs, s, f, crash_error)
+            else (hs, s, f, crash_error))
+          (hs, s, f, crash_error)
+      else (hs, s, f, crash_error)
+    | Basic (EConst _) => (hs, s, f, crash_error)
     | Invoke cl =>
       match cl with
-      | Func_native i' (Tf t1s t2s) ts es =>
+      | Func_native i (Tf t1s t2s) ts es =>
         let: n := length t1s in
         let: m := length t2s in
         if length ves >= n
         then
           let: (ves', ves'') := split_n ves n in
           let: zs := n_zeros ts in
-          (hs, s, vs, RS_normal (vs_to_es ves''
-                  ++ [::Local m i' (rev ves' ++ zs) [::Basic (Block (Tf [::] t2s) es)]]))
-        else (hs, s, vs, crash_error)
-      | Func_host (Tf t1s t2s) f =>
+          (hs, s, f, RS_normal (vs_to_es ves''
+                  ++ [::Local m (Build_frame (rev ves' ++ zs) i) [::Basic (Block (Tf [::] t2s) es)]]))
+        else (hs, s, f, crash_error)
+      | Func_host (Tf t1s t2s) cl' =>
         let: n := length t1s in
         let: m := length t2s in
         if length ves >= n
         then
           let: (ves', ves'') := split_n ves n in
-          match host_application_impl hs s (Tf t1s t2s) f (rev ves') with
+          match host_application_impl hs s (Tf t1s t2s) cl' (rev ves') with
           | (hs', Some (s', rves)) =>
-            (hs', s', vs, RS_normal (vs_to_es ves'' ++ (result_to_stack rves)))
-        | (hs', None) => (hs', s, vs, RS_normal (vs_to_es ves ++ [::Invoke cl]))
+            (hs', s', f, RS_normal (vs_to_es ves'' ++ (result_to_stack rves)))
+        | (hs', None) => (hs', s, f, RS_normal (vs_to_es ves ++ [::Invoke cl]))
           end
-        else (hs, s, vs, crash_error)
+        else (hs, s, f, crash_error)
       end
     | Label ln les es =>
       if es_is_trap es
-      then (hs, s, vs, RS_normal (vs_to_es ves ++ [::Trap]))
+      then (hs, s, f, RS_normal (vs_to_es ves ++ [::Trap]))
       else
         if const_list es
-        then (hs, s, vs, RS_normal (vs_to_es ves ++ es))
+        then (hs, s, f, RS_normal (vs_to_es ves ++ es))
         else
-          let: (hs', s', vs', res) := run_step_with_fuel fuel d i (hs, s, vs, es) in
+          let: (hs', s', f', res) := run_step_with_fuel fuel d (hs, s, f, es) in
           match res with
           | RS_break 0 bvs =>
             if length bvs >= ln
-            then (hs', s', vs', RS_normal ((vs_to_es ((take ln bvs) ++ ves)) ++ les))
-            else (hs', s', vs', crash_error)
-          | RS_break (n.+1) bvs => (hs', s', vs', RS_break n bvs)
-          | RS_return rvs => (hs', s', vs', RS_return rvs)
+            then (hs', s', f', RS_normal ((vs_to_es ((take ln bvs) ++ ves)) ++ les))
+            else (hs', s', f', crash_error)
+          | RS_break (n.+1) bvs => (hs', s', f', RS_break n bvs)
+          | RS_return rvs => (hs', s', f', RS_return rvs)
           | RS_normal es' =>
-            (hs', s', vs', RS_normal (vs_to_es ves ++ [::Label ln les es']))
-          | RS_crash error => (hs', s', vs', RS_crash error)
+            (hs', s', f', RS_normal (vs_to_es ves ++ [::Label ln les es']))
+          | RS_crash error => (hs', s', f', RS_crash error)
           end
-    | Local ln j vls es =>
+    | Local ln lf es =>
       if es_is_trap es
-      then (hs, s, vs, RS_normal (vs_to_es ves ++ [::Trap]))
+      then (hs, s, f, RS_normal (vs_to_es ves ++ [::Trap]))
       else
         if const_list es
         then
           if length es == ln
-          then (hs, s, vs, RS_normal (vs_to_es ves ++ es))
-          else (hs, s, vs, crash_error)
+          then (hs, s, f, RS_normal (vs_to_es ves ++ es))
+          else (hs, s, f, crash_error)
         else
-          let: (hs', s', vls', res) := run_step_with_fuel fuel d j (hs, s, vls, es) in
+          let: (hs', s', f', res) := run_step_with_fuel fuel d (hs, s, lf, es) in
           match res with
           | RS_return rvs =>
             if length rvs >= ln
-            then (hs', s', vs, RS_normal (vs_to_es (take ln rvs ++ ves)))
-            else (hs', s', vs, crash_error)
+            then (hs', s', f, RS_normal (vs_to_es (take ln rvs ++ ves)))
+            else (hs', s', f, crash_error)
           | RS_normal es' =>
-            (hs', s', vs, RS_normal (vs_to_es ves ++ [::Local ln j vls' es']))
-          | RS_crash error => (hs', s', vs, RS_crash error)
-          | RS_break _ _ => (hs', s', vs, crash_error)
+            (hs', s', f, RS_normal (vs_to_es ves ++ [::Local ln f' es']))
+          | RS_crash error => (hs', s', f, RS_crash error)
+          | RS_break _ _ => (hs', s', f, crash_error)
           end
-    | Trap => (hs, s, vs, crash_error)
+    | Trap => (hs, s, f, crash_error)
     end
   end.
 
@@ -487,14 +487,14 @@ Defined.
 
 (** Enough fuel so that [run_step] does not run out of exhaustion. **)
 Definition run_step_fuel (cfg : config_tuple) : nat :=
-  let: (hs, s, vs, es) := cfg in
+  let: (hs, s, f, es) := cfg in
   1 + List.fold_left max (List.map run_one_step_fuel es) 0.
 
-Definition run_step (d : depth) (inst : instance) (cfg : config_tuple) : res_tuple :=
-  run_step_with_fuel (run_step_fuel cfg) d inst cfg.
+Definition run_step (d : depth) (cfg : config_tuple) : res_tuple :=
+  run_step_with_fuel (run_step_fuel cfg) d cfg.
 
-Fixpoint run_v (fuel : fuel) (d : depth) (i : instance) (cfg : config_tuple) : ((host_state * store_record * res)%type) :=
-  let: (hs, s, vs, es) := cfg in
+Fixpoint run_v (fuel : fuel) (d : depth) (cfg : config_tuple) : ((host_state * store_record * res)%type) :=
+  let: (hs, s, f, es) := cfg in
   match fuel with
   | 0 => (hs, s, R_crash C_exhaustion)
   | fuel.+1 =>
@@ -504,9 +504,9 @@ Fixpoint run_v (fuel : fuel) (d : depth) (i : instance) (cfg : config_tuple) : (
       if const_list es
       then (hs, s, R_value (fst (split_vals_e es)))
       else
-        let: (hs', s', vs', res) := run_step d i (hs, s, vs, es) in
+        let: (hs', s', f', res) := run_step d (hs, s, f, es) in
         match res with
-        | RS_normal es' => run_v fuel d i (hs', s', vs', es')
+        | RS_normal es' => run_v fuel d (hs', s', f', es')
         | RS_crash error => (hs', s', R_crash error)
         | _ => (hs', s', R_crash C_error)
         end
